save

experiments/coq-experiments/proplang/PerfFuzz/Analysis.py
@@ -1,0 +1,81 @@
+import pathlib
+from typing import List
+import random
+from benchtool.Analysis import *
+from benchtool.Plot import *
+from functools import partial
+import itertools
+
+def df_insert(df: pd.DataFrame, column: str, value: any) -> pd.DataFrame:
+    df.insert(len(df.columns), column, value)
+    return df
+
+def parse_results(results: str) -> pd.DataFrame:
+    entries = scandir_filter(results, os.path.isfile)
+    entries = [e for e in entries if e.path.endswith('.json')]
+
+    df = pd.concat([df_insert(pd.read_json(e.path, orient='records', typ='frame'), "version", e.name.split(',')[2]) for e in entries])
+
+    df['inputs'] = df.apply(lambda x: x['passed'] + (1 if x['foundbug'] else 0), axis=1)
+    df = df.drop(['passed'], axis=1)
+
+    df['task'] = df['workload'] + ',' + df['mutant'] + ',' + df['property']
+    return df
+
+
+def insertion_sort(ls: List[int]) -> int:
+    num_comparisons = 0
+    for i in range(1, len(ls)):
+        j = i
+        while j > 0 and ls[j] < ls[j-1]:
+            num_comparisons += 1
+            ls[j], ls[j-1] = ls[j-1], ls[j]
+            j -= 1
+    return num_comparisons
+
+def mkList(s: str) -> List[int]:
+    try:
+        stripped = s[4:-1]
+        nums = stripped.split('; ')
+        return [int(n) for n in nums]
+    except Exception as e:
+        return []
+
+
+def insertion_sort_on_random_lists() -> float:
+    sum = 0
+    n = 100
+    for i in range(n):
+        ls = [random.randint(0, 10) for _ in range(1000)]
+        sum += (insertion_sort(ls) / (len(ls) ** 2))
+    return sum / n 
+
+def insertion_sort_on_reverse_sorted_lists() -> float:
+    sum = 0
+    n = 100
+    for i in range(n):
+        ls = list(range(1000, 0, -1))
+        sum += (insertion_sort(ls) / (len(ls) ** 2))
+    return sum / n
+
+if __name__ == "__main__":
+
+    filepath = pathlib.Path(__file__).resolve().parent
+
+    results_path = f'{filepath}/results'
+    images_path = f'{filepath}/figures'
+
+    df = parse_results(results_path)
+
+    df['comparisons'] = df['counterexample'].apply(mkList).apply(insertion_sort)
+    df['lengths'] = df['counterexample'].apply(mkList).apply(len)
+    df['comp/lens^2'] = df['comparisons'] / (df['lengths'] ** 2)
+
+    df = df.drop(['workload', 'discards', 'foundbug', 'strategy', 'mutant', 'property', 'version', 'task', 'time', 'counterexample'], axis=1)
+
+    df.to_csv(f'{results_path}/results.csv')
+
+
+    print(df.groupby('inputs').mean())
+
+    
