workloads/Coq/SortingProplang/Src/Impl.v
@@ -1,0 +1,22 @@
+
+Require Import List.
+Import ListNotations.
+
+Require Import Nat.
+Local Open Scope nat.
+Local Open Scope nat_scope.
+
+Require Import Bool.
+Import BoolNotations.
+
+Fixpoint insert (i : nat) (l : list nat) :=
+  match l with
+  | [] => [i]
+  | h :: t => if Nat.leb i h then i :: h :: t else h :: insert i t
+  end.
+
+Fixpoint sort (l : list nat) : list nat :=
+  match l with
+  | [] => []
+  | h :: t => insert h (sort t)
+  end.
